src/proofs/Gen/TermTactics.v
@@ -3,3 +3,7 @@
 Ltac destruct_term_node t:=
   let n := fresh "n" in
   destruct t as [n ? ? ?]; destruct n; try discriminate; simpl in *; subst; simpl in *.
+
+Ltac destruct_pat_node p :=
+  let n := fresh "n" in
+  destruct p as [n ? ?]; destruct n; try discriminate; simpl in *; subst; simpl in *.
